current

examples/low-level/crypto/Crypto.Symmetric.GF128.Spec.fst
@@ -7,12 +7,23 @@ module U128 = FStar.UInt128
 type text = Seq.seq (lbytes 16)
 type elem = U128.t
 
-assume val op_Plus_At: elem -> elem -> Tot elem
-assume val op_Star_At: elem -> elem -> Tot elem
+val op_Plus_At: elem -> elem -> Tot elem
+let op_Plus_At x y = U128.(x ^^ y)
+
+val op_Star_At: elem -> elem -> Tot elem
+let op_Star_At x y = U128.(x ^^ y) // FAKE IMPLEMENTATION TODO FIX
 
 assume val add_comm: a:elem -> b:elem -> Lemma (a +@ b == b +@ a)
 
-assume val zero: elem
+val zero: elem
+let zero = FStar.Int.Cast.uint64_to_uint128(0uL)
+
+val encode:lbytes 16 -> Tot elem
+let encode b = zero // FAKE IMPLEMENTATION TODO FIX
+val decode:elem -> Tot (lbytes 16)
+let decode e = Seq.create 16 0uy
+
+
 
 (*
 val add_loop: l:nat -> lbytes l -> lbytes l -> Tot (lbytes l)
@@ -33,8 +44,6 @@ open FStar.SeqProperties
 
 let seq_head (vs:seq 'a {Seq.length vs > 0}) = Seq.slice vs 0 (Seq.length vs - 1)
 
-assume val encode:lbytes 16 -> Tot elem
-assume val decode:elem -> Tot (lbytes 16)
 
 val poly: vs:text -> r:elem -> Tot (a:elem) (decreases (Seq.length vs))
 let rec poly vs r =
